<div align="center"> 
$\frac{dp}{dx}=\frac{\left ( P1-P2 \right )}{L}$ 
</div>

<div align="center"> 
$Q=\int (\vec{V}*dA)$
</div>

<div align="center"> 
$\tau=\gamma *R*S_f$
</div>

<div align="center"> 
$R_e=\frac{\rho *\bar{V}*D}{\mu}$
</div>

<div align="center"> 
$Q= V*A$
</div>

<div align="center"> 
$\sum Qentrada-\sum Qsalida = \frac{dV}{dt}$
</div>

<div align="center"> 
$\sum Qentrada-\sum Qsalida = 0$
</div>

<div align="center"> 
$\frac{dQ}{dt}-\frac{dW}{dt}=\frac{dE}{dt}$

</div>

<div align="center"> 
$m\dot{}=Q*\rho$
</div>

<div align="center"> 
$\sum_{}Q*\rho_{entrada}-\sum_{}Q*\rho_{salida}=0$
</div>

<div align="center"> 
$Q = \frac{\pi*g*D^4*\Delta(P/\gamma)}{128*\vartheta*L}$
</div>

<div align="center"> 
$Q=0.849*C*R^{0.63}*Sf^{0.54}*A$
</div>

<div align="center"> 
$\frac{V^{2}_1}{2g}+Z_1+\frac{P_1}{\gamma}=\frac{V^{2}_2}{2g}+Z_2+\frac{P_2}{\gamma}$
</div>

<div align="center"> 
$\frac{V^{2}_1}{2g}+Z_1+\frac{P_1}{\gamma}-\sum_{}^{}\Delta h_f-\sum_{}^{}\Delta h_k=\frac{V^{2}_2}{2g}+Z_2+\frac{P_2}{\gamma}$
</div>

<div align="center"> 
$H_p=\frac{P_w}{Q*\gamma}$
</div>

<div align="center"> 
$h_{f}=\frac{f*L}{D}*\frac{V^{2}}{2g}$
</div>

<div align="center"> 
$f= \frac{64}{Re}$
</div>

<div align="center"> 
$\frac{1}{\sqrt{f}}=-2*Log (\frac{\frac{\epsilon}{D}}{3.7}+\frac{2.51}{Re\sqrt{f}})$
</div>

<div align="center"> 
$h_k=K*\frac{V^2}{2g}$
</div> 

<div align="center"> 
$K = C_a *(\frac{A_2}{A_1}-1)^2$
</div>

<div align="center"> 
$K = (\frac{A_2}{A_1}-1)^2$
</div>

<div align="center"> 
$h_s=K*\frac{(V_s-V_2)^2}{2*g}$
</div>

<div align="center"> 
$\frac{V^{2}_1}{2g}+\frac{P_1}{\gamma}+h_p=\frac{V^{2}_2}{2g}+\frac{P_2}{\gamma}$
</div>

<div align="center"> 
$h_p=\frac{V^{2}_2-V^{2}_1}{2g}-\frac{P_2-P_1}{\gamma}$
</div>

<div align="center"> 
$h_p=\frac{(\frac{Q}{A_2})^{2}-(\frac{Q}{A_1})^{2}}{2g}-\frac{P_2-P_1}{\gamma}$
</div>

<div align="center"> 
$P_h=\gamma*Q*H_p$
</div>

<div align="center"> 
$P_m=T*\omega$
</div>

<div align="center"> 
$P_E=I*V$
</div>

<div align="center">
$\eta= \frac{P_h}{P_m}$
</div>

<div align="center">
$\eta_e= \frac{P_m}{P_e}$
</div>

<div align="center">
$EAS=\frac{P_atm}{\gamma}\pm h_s - h_f$
</div>

<div align="center">
$(EAS)_D=EAS-PV$
</div>

<div align="center"> 
$h_t=\frac{V^{2}_2-V^{2}_1}{2g}-\frac{P_2-P_1}{\gamma}+\sum_{}^{}h_k+\sum_{}^{}h_f$
</div>

<div align="center">
$\sum_{i=1}^{n}Q_i=0$
</div>

<div align="center"> 
$\frac{V^{2}_1}{2g}+Z_1+\frac{P_1}{\gamma}-\sum_{}^{}\Delta h_f-\sum_{}^{}\Delta h_k=\frac{V^{2}_2}{2g}+Z_2+\frac{P_2}{\gamma}$
</div>

<div align="center"> 
$\frac{V^{2}_2}{2g}+Z_2+\frac{P_2}{\gamma}-\sum_{}^{}\Delta h_f-\sum_{}^{}\Delta h_k=\frac{V^{2}_a}{2g}+Z_a+\frac{P_a}{\gamma}$
</div>

<div align="center"> 
$\frac{V^{2}_3}{2g}+Z_3+\frac{P_3}{\gamma}-\sum_{}^{}\Delta h_f-\sum_{}^{}\Delta h_k=\frac{V^{2}_a}{2g}+Z_a+\frac{P_a}{\gamma}$
</div>

<div align="center"> 
$\frac{V^{2}_a}{2g}+Z_a+\frac{P_a}{\gamma}-\sum_{}^{}\Delta h_f-\sum_{}^{}\Delta h_k=\frac{V^{2}_4}{2g}+Z_4+\frac{P_4}{\gamma}$
</div>

<div align="center"> 
$\sum_{}^{}h_f+\sum_{}^{}h_k=\sum_{}^{}\frac{F_i*L_i}{2g}*\frac{V_i^2}{2g}+\sum_{}^{}K_i*\frac{V_i^2}{2g}$
</div>

<div align="center"> 
$Le=\sum_{i=1}^{n}\frac{K_i*D_i}{F_i}$
</div>

<div align="center"> 
$L_e=\sum_{}^{}\frac{F_i*(Lt+L_e)_i}{2g}*\frac{V_i^2}{2g}$
</div>

<div align="center"> 
$hf_i=a_i*Q^2_i$
</div>

<div align="center"> 
$a_i=\frac{8*f_i*L_i}{\pi^2*g*D_i^2}$
</div>

<div align="center"> 
$\Delta Q= \frac{\sum_{i=1}^{n}(a_i*Q^{N-1}_i*\left|Q_i \right|)}{N*\sum_{i=1}^{n}(a_i*Q^{N-1}_i)}$
</div>

<div align="center"> 
$\Delta H_i=-N*(\frac{Q_i+\sum_{i=1}^{n}Q_i}{\sum_{i=1}^{n}(Q_i/h_i)})$
</div>

<div align="center"> 
$Z_1-\sum_{}^{}\Delta h_{f_{1-a}}=\frac{V^{2}_a}{2g}+Z_a+\frac{P_a}{\gamma}$
</div>

<div align="center"> 
$Z_a+\frac{P_a}{\gamma}+\frac{V^{2}_a}{2g}-\sum_{}^{}\Delta h_{f_{a-3}}=Z_3$
</div>

<div align="center"> 
$\sum_{i=1}^{n}Q_i=0$
</div>